\chapter{Sistemi lineari}
\section{Sostituzione}
\tcbstartrecording
\begin{exercise}{}
Risolvere il sistema 
\[
\begin{cases}
	x+3y=5\\
	2x+y=6
\end{cases}
\]
	\tcblower
\[
\begin{cases}
	x+3y=5\\
	2x+y=6
\end{cases}
\begin{cases}
	x=5-3y\\
	2(5-3y)+y=6
\end{cases}
\begin{cases}
	x=5-3y\\
	10-6y+y=6
\end{cases}
\begin{cases}
	x=5-3y\\
	-5y=-10+6
\end{cases}
\]
\[
\begin{cases}
		x=5-3y\\
	-5y=-4
\end{cases}
\begin{cases}
	x=5-3y\\
	y=\dfrac{4}{5}
\end{cases}
\begin{cases}
	x=5-3\dfrac{4}{5}\\
	y=\dfrac{4}{5}
\end{cases}
\begin{cases}
	x=5-\dfrac{12}{5}\\
	y=\dfrac{4}{5}
\end{cases}
\begin{cases}
	x=\dfrac{25-12}{5}\\
	y=\dfrac{4}{5}
\end{cases}
\begin{cases}
	x=\dfrac{13}{5}\\
	y=\dfrac{4}{5}
\end{cases}
\]
\end{exercise}
\begin{exercise}[no solution]
Risolvere il sistema 
\[
\begin{cases}
	x+y=-1\\
	2x+3y=6
\end{cases}
\]
\end{exercise}
\begin{exercise}[no solution]
	Risolvere il sistema 
	\[
	\begin{cases}
		3x+y=-3\\
		2x-3y=6
	\end{cases}
	\]
\end{exercise}
\begin{exercise}{}
	Risolvere il sistema 
	\[
	\begin{cases}
		x+y=1\\
		x-y=1
	\end{cases}
	\]
	\tcblower
	\[
	\begin{cases}
		x+y=1\\
		x-y=1
	\end{cases}
	\begin{cases}
		x=1-y\\
		1-y-y=1
	\end{cases}
	\begin{cases}
		x=1-y\\
		-2y=0
	\end{cases}
	\begin{cases}
	x=1-y\\
	y=0
	\end{cases}
	\]
	\[
	\begin{cases}
		x=1\\
		y=0
	\end{cases}
	\]
\end{exercise}
\begin{exercise}{}
	Risolvere il sistema 
	\[
	\begin{cases}
		\dfrac{1}{2}x+y=5\\
		x-\dfrac{2}{3}y=0
	\end{cases}
	\]
	\tcblower
	\[
	\begin{cases}
		\dfrac{1}{2}x+y=5\\
	x-\dfrac{2}{3}y=0
	\end{cases}
\begin{cases}
	\tikzmark{1}\dfrac{1}{2}x+y=5\\
	\tikzmark{2}x-\dfrac{2}{3}y=0
\end{cases}
\begin{tikzpicture}[remember picture, overlay]
	\node[left=2cm and 0cm of 1](3){$2$};
	\node[left=2cm and 0cm of 2](4){$3$};
\end{tikzpicture}\\
\begin{cases}
	\dfrac{2}{2}x+2y=10\\
	3x-\dfrac{6}{3}y=0
\end{cases}
\begin{cases}
	x+2y=10\\
	3x-2y=0
\end{cases}
\begin{cases}
	x=10-2y\\
	3(10-2y)-2y=0
\end{cases}
	\]
	\[
	\begin{cases}
		x=10-2y\\
		30-6y-2y=0
	\end{cases}
\begin{cases}
	x=10-2y\\
	30-6y-2y=0
\end{cases}
\begin{cases}
	x=10-2y\\
	-8y=-30
\end{cases}
\begin{cases}
	x=10-2y\\
	y=\dfrac{30}{8}
\end{cases}
\begin{cases}
	x=10-2y\\
	y=\dfrac{15}{4}
\end{cases}
	\]
	\[
	\begin{cases}
		x=10-2\dfrac{15}{4}\\
		y=\dfrac{15}{4}
	\end{cases}
\begin{cases}
	x=10-\dfrac{15}{2}\\
	y=\dfrac{15}{4}
\end{cases}
\begin{cases}
	x=\dfrac{20-15}{2}\\
	y=\dfrac{15}{4}
\end{cases}
\begin{cases}
	x=\dfrac{5}{2}\\
	y=\dfrac{15}{4}
\end{cases}
	\]
\end{exercise}
\section{Confronto}
\begin{exercise}{}
	Risolvere il sistema 
	\[
	\begin{cases}
		x+2y=0\\
		x-4y=2
	\end{cases}
	\]
	\tcblower
	\[
	\begin{cases}
		x+2y=0\\
	x-4y=2
	\end{cases}
	\begin{cases}
		x=-2y\\
	x=4y+2
	\end{cases}
	\begin{cases}
		x=-2y\\
	x=4y+2
	\end{cases}
	\begin{cases}
		-2y=4y+2\\
		x=-2y
	\end{cases}
\begin{cases}
	-2y-4y=2\\
	x=-2y
\end{cases}
\]
	\[
	\begin{cases}
		-6y=2\\
		x=-2y
	\end{cases}
	\begin{cases}
		y=-\dfrac{2}{6}\\
		x=-2y
	\end{cases}
	\begin{cases}
	y=-\dfrac{1}{3}\\
	x=-2y
	\end{cases}
\begin{cases}
	y=-\dfrac{1}{3}\\
	x=-2(-\dfrac{1}{3})
\end{cases}
\begin{cases}
	y=-\dfrac{1}{3}\\
	x=\dfrac{2}{3}
\end{cases}
	\]
\end{exercise}
\begin{exercise}{}
	Risolvere il sistema 
	\[
	\begin{cases}
		2x-y=3\\
		5x-y=-6
	\end{cases}
	\]
	\tcblower
	\[
	\begin{cases}
		2x-y=3\\
		5x-y=-6
	\end{cases}
	\begin{cases}
	-y=3-2x\\
	-y=-6-5x
	\end{cases}
	\begin{cases}
	y=-3+2x\\
	y=+6+5x
	\end{cases}
	\begin{cases}
	-3+2x=+6+5x\\
		y=+6+5x
	\end{cases}
\]
\[
	\begin{cases}
2x-5x=+6+3\\
	y=+6+5x
	\end{cases}
\begin{cases}
	-3x=9\\
	y=+6+5x
\end{cases}
\begin{cases}
	x=-3\\
	y=+6+5x
\end{cases}
\begin{cases}
	x=-3\\
	y=+6-15
\end{cases}
\begin{cases}
	x=-3\\
	y=-9
\end{cases}
	\]
\end{exercise}
\begin{exercise}{}
	Risolvere il sistema 
	\[
	\begin{cases}
		x+2y=3\\
		2x+y=4
	\end{cases}
	\]
	\tcblower
	\[
	\begin{cases}
		x+2y=3\\
	2x+y=4
	\end{cases}
\begin{cases}
	2y=3-x\\
	y=-2x+4
\end{cases}
\begin{cases}
	y=\dfrac{3-x}{2}\\
	y=-2x+4
\end{cases}
\begin{cases}
	\dfrac{3-x}{2}=	y=-2x+4\\
	y=-2x+4
\end{cases}
		\]
	\[
	\begin{cases}
		\tikzmark{1}\dfrac{3-x}{2}=-2x+4\\
		y=-2x+4
	\end{cases}
	\begin{tikzpicture}[remember picture, overlay]
		\node[left=2cm and 0cm of 1](3){$2$};
	\end{tikzpicture}
		\begin{cases}
		\dfrac{2(3-x)}{2}=2(-2x+4)\\
		y=-2x+4
	\end{cases}
	\begin{cases}
	3-x=-4x+8\\
	y=-2x+4
\end{cases}
\begin{cases}
	-x+4x=-3+8\\
	y=-2x+4
\end{cases}
\]
\[
\begin{cases}
	3x=5\\
	y=-2x+4
\end{cases}
\begin{cases}
	x=\dfrac{5}{3}\\
	y=-2x+4
\end{cases}
\begin{cases}
	x=\dfrac{5}{3}\\
	y=-2\dfrac{5}{3}+4
\end{cases}
\begin{cases}
	x=\dfrac{5}{3}\\
	y=-\dfrac{10}{3}+4
\end{cases}
	\]
	\[
	\begin{cases}
		x=\dfrac{5}{3}\\
		y=\dfrac{-10+12}{3}
	\end{cases}
	\begin{cases}
	x=\dfrac{5}{3}\\
	y=\dfrac{2}{3}
\end{cases}
	\]
\end{exercise}
\begin{exercise}{}
	Risolvere il sistema 
	\[
	\begin{cases}
		2x+3y=1\\
		3x+2y=-3
	\end{cases}
	\]
	\tcblower
	\[
	\begin{cases}
		2x+3y=1\\
	3x+2y=-3
	\end{cases}
	\begin{cases}
			2x=1-3y\\
		3x=-3-2x
	\end{cases}
	\begin{cases}
		x=\dfrac{1-3y}{2}\\
		x=\dfrac{-2y-3}{3}
	\end{cases}
	\begin{cases}
		\dfrac{1-3y}{2}=\dfrac{-2y-3}{3}\\
	x=\dfrac{1}{2}-\dfrac{3}{2}y
	\end{cases}
	\]
	\[
	\begin{cases}
		\tikzmark{1}\dfrac{1-3y}{2}=\dfrac{-2y-3}{3}\\
	x=\dfrac{1}{2}-\dfrac{3}{2}y
	\end{cases}
	\begin{tikzpicture}[remember picture, overlay]
		\node[left=2cm and 0cm of 1](3){$6$};
	\end{tikzpicture}
	\begin{cases}
	\dfrac{6(1-3y)}{2}=\dfrac{6(-2y-3)}{3}\\
	x=\dfrac{1}{2}-\dfrac{3}{2}y
	\end{cases}
	\begin{cases}
		3(1-3y)=2(-2y-3)\\
		x=\dfrac{1}{2}-\dfrac{3}{2}y
	\end{cases}
	\begin{cases}
		3-9y=-4y-6\\
		x=\dfrac{1}{2}-\dfrac{3}{2}y
	\end{cases}
	\]
	\[
	\begin{cases}
		-9y+4y=-3-6\\
		x=\dfrac{1}{2}-\dfrac{3}{2}y
	\end{cases}
	\begin{cases}
		-5y=-9\\
		x=\dfrac{1}{2}-\dfrac{3}{2}y
	\end{cases}
	\begin{cases}
		y=\dfrac{9}{5}\\
		x=\dfrac{1}{2}-\dfrac{3}{2}y
	\end{cases}
	\begin{cases}
		y=\dfrac{9}{5}\\
		x=\dfrac{1}{2}-\dfrac{3}{2}\dfrac{9}{5}
	\end{cases}
	\]
	\[
	\begin{cases}
		y=\dfrac{9}{5}\\
			x=\dfrac{1}{2}-\dfrac{27}{10}
	\end{cases}
	\begin{cases}
			y=\dfrac{9}{5}\\
		x=\dfrac{5-27}{10}
	\end{cases}
\begin{cases}
	y=\dfrac{9}{5}\\
	x=-\dfrac{22}{10}
\end{cases}
\begin{cases}
	y=\dfrac{9}{5}\\
	x=-\dfrac{11}{5}
\end{cases}
	\]
\end{exercise}
\tcbstoprecording
\newpage
\chapter{Soluzioni esercizi}
\tcbinputrecords